memory_map.v
@@ -9,33 +9,33 @@ Section operations.
   Global Instance cmap_dom: Dom (mem Ti) indexset := λ m,
     let (m) := m in dom _ m.
   Global Instance cmap_valid: Valid (env Ti) (mem Ti) := λ Γ m,
-    map_Forall (λ _ w, ∃ τ,
-      (**i 1). *) (Γ,m) ⊢ w : τ ∧
-      (**i 2). *) ¬ctree_empty w ∧
+    map_Forall (λ _ wβ, ∃ τ,
+      (**i 1). *) (Γ,m) ⊢ wβ.1 : τ ∧
+      (**i 2). *) ¬ctree_empty (wβ.1) ∧
       (**i 3). *) int_typed (size_of Γ τ) sptrT
     ) (cmap_car m).
   Global Instance cmap_lookup:
       LookupE (env Ti) (addr Ti) (mtree Ti) (mem Ti) := λ Γ a m,
     guard (addr_strict Γ a);
-    w ← cmap_car m !! addr_index a ≫= lookupE Γ (addr_ref Γ a);
+    w ← cmap_car m !! addr_index a ≫= lookupE Γ (addr_ref Γ a) ∘ fst;
     if decide (addr_is_obj a) then Some w else
       guard (ctree_unshared w ∧ type_of a ≠ voidT); w !!{Γ} (addr_ref_byte Γ a).
   Definition cmap_alter (Γ : env Ti) (g : mtree Ti → mtree Ti)
       (a : addr Ti) (m : mem Ti) : mem Ti :=
-    let (m) := m in CMap $ alter (ctree_alter Γ (λ w,
+    let (m) := m in CMap $ alter (prod_map (ctree_alter Γ (λ w,
       if decide (addr_is_obj a) then g w
       else ctree_alter_byte Γ g (addr_ref_byte Γ a) w
-    ) (addr_ref Γ a)) (addr_index a) m.
+    ) (addr_ref Γ a)) id) (addr_index a) m.
 
   Global Instance cmap_refine: RefineM Ti (mem Ti) := λ Γ f m1 m2,
     (**i 1.) *) mem_inj_injective f ∧
     (**i 2.) *) ✓{Γ} m1 ∧
     (**i 3.) *) ✓{Γ} m2 ∧
-    (**i 4.) *) ∀ o1 o2 r w1,
-      f !! o1 = Some (o2,r) → cmap_car m1 !! o1 = Some w1 →
-      ∃ w2 w2' τ, cmap_car m2 !! o2 = Some w2 ∧
+    (**i 4.) *) ∀ o1 o2 r w1 (β : bool),
+      f !! o1 = Some (o2,r) → cmap_car m1 !! o1 = Some (w1,β) →
+      ∃ w2 w2' τ, cmap_car m2 !! o2 = Some (w2,β) ∧
         w2 !!{Γ} (freeze true <$> r) = Some w2' ∧
-        w1 ⊑{Γ,f@m1↦m2} w2' : τ.
+        w1 ⊑{Γ,f@m1↦m2} w2' : τ ∧ (β → r = []).
 End operations.
 
 Section cmap_typed.
@@ -50,6 +50,7 @@ Implicit Types r : ref Ti.
 Implicit Types a : addr Ti.
 Implicit Types f : mem_inj Ti.
 Implicit Types g : mtree Ti → mtree Ti.
+Implicit Types β : bool.
 
 Arguments lookupE _ _ _ _ _ _ _ !_ /.
 Arguments cmap_lookup _ _ _ _ _ !_ /.
@@ -58,16 +59,16 @@ Hint Extern 0 (Separation _) => apply (_ : Separation (pbit Ti)).
 Global Instance mem_index_alive_dec m o : Decision (index_alive m o).
 Proof.
  refine
-  match cmap_car m !! o as mo return Decision (∃ w, mo = Some w ∧ _) with
-  | Some w =>
-     cast_if_not (decide (ctree_Forall (λ xb, tagged_perm xb = perm_freed) w))
+  match cmap_car m !! o as mo return Decision (∃ wβ, mo = Some wβ ∧ _) with
+  | Some wβ =>  cast_if_not
+     (decide (ctree_Forall (λ xb, tagged_perm xb = perm_freed) (wβ.1)))
   | _ => right _
   end; abstract naive_solver.
 Defined.
 Lemma index_typed_alt m o τ :
-  m ⊢ o : τ ↔ ∃ w, cmap_car m !! o = Some w ∧ τ = type_of w.
+  m ⊢ o : τ ↔ ∃ wβ, cmap_car m !! o = Some wβ ∧ τ = type_of (wβ.1).
 Proof.
-  change (m ⊢ o : τ) with (type_of <$> cmap_car m !! o = Some τ).
+  change (m ⊢ o : τ) with (type_of ∘ fst <$> cmap_car m !! o = Some τ).
   destruct (cmap_car m !! o); naive_solver.
 Qed.
 Lemma cmap_empty_valid Γ : ✓{Γ} (∅ : mem Ti).
@@ -102,7 +103,7 @@ Proof.
   rewrite addr_index_freeze, addr_ref_freeze, addr_ref_byte_freeze.
   case_option_guard; simplify_equality'.
   rewrite option_guard_True by auto using addr_strict_freeze_2.
-  destruct (m !! addr_index a) as [w'|]; simplify_equality'.
+  destruct (m !! addr_index a) as [[w' β]|]; simplify_equality'.
   destruct (w' !!{Γ} addr_ref Γ a) as [w''|] eqn:?; simplify_equality'.
   erewrite ctree_lookup_unfreeze by eauto; csimpl.
   by rewrite (decide_iff _ _ _ _ (addr_is_obj_freeze _ _)), addr_type_of_freeze.
@@ -112,15 +113,16 @@ Lemma cmap_lookup_typed Γ m a w σ :
 Proof.
   destruct m as [m]; simpl; intros ? Hm Ha ?.
   case_option_guard; simplify_equality'.
-  destruct (m !! addr_index a) as [w'|] eqn:Hw; simplify_equality'.
+  destruct (m !! addr_index a) as [[w' β]|] eqn:Hw; simplify_equality'.
   destruct (w' !!{Γ} addr_ref Γ a) as [w''|] eqn:?; simplify_equality'.
-  destruct (Hm (addr_index a) w' Hw) as (τ&Hoτ&_); simplify_equality'.
+  destruct (Hm (addr_index a) (w',β) Hw) as (τ&Hoτ&_); simplify_equality'.
   destruct (ctree_lookup_Some Γ (CMap m) w' τ (addr_ref Γ a) w'')
     as (σ'&?&?); auto; simplify_option_equality; simplify_type_equality.
   * cut (σ = σ'); [by intros ->|].
     erewrite <-(addr_is_obj_type_base _ _ _ σ) by eauto.
-    assert (∃ w, m !! addr_index a = Some w ∧ addr_type_object a = type_of w) 
-     as (?&?&?) by (eapply (index_typed_alt (CMap m)), addr_typed_index; eauto).
+    assert (∃ wβ, m !! addr_index a = Some wβ ∧
+      addr_type_object a = type_of (wβ.1)) as (?&?&?)
+      by (eapply (index_typed_alt (CMap m)), addr_typed_index; eauto).
     simplify_type_equality'.
     eauto using ref_set_offset_typed_unique, addr_typed_ref_base_typed.
   * erewrite addr_not_obj_type by intuition eauto.
@@ -133,9 +135,9 @@ Lemma cmap_lookup_Some Γ m w a :
 Proof.
   destruct m as [m]; simpl; intros ? Hm Ha.
   case_option_guard; simplify_equality'.
-  destruct (m !! addr_index a) as [w'|] eqn:Hw; simplify_equality'.
+  destruct (m !! addr_index a) as [[w' β]|] eqn:Hw; simplify_equality'.
   destruct (w' !!{Γ} addr_ref Γ a) as [w''|] eqn:?; simplify_equality'.
-  destruct (Hm (addr_index a) w' Hw) as (τ&Hoτ&_); simplify_equality'.
+  destruct (Hm (addr_index a) (w',β) Hw) as (τ&Hoτ&_); simplify_equality'.
   destruct (ctree_lookup_Some Γ (CMap m) w' τ (addr_ref Γ a) w'')
     as (σ'&?&?); auto; simplify_option_equality;
     eauto using ctree_lookup_byte_typed, type_of_typed.
@@ -147,12 +149,12 @@ Proof.
   destruct m1 as [m1], m2 as [m2]; simpl.
   intros ? Hm1 Hm2 Hm ??. case_option_guard; simplify_equality'.
   specialize (Hm (addr_index a)).
-  destruct (m1 !! addr_index a) as [w1'|] eqn:Hw1; simplify_equality'.
-  destruct (m2 !! addr_index a) as [w2'|] eqn:Hw2; simplify_equality'.
+  destruct (m1 !! addr_index a) as [[w1' β]|] eqn:Hw1; simplify_equality'.
+  destruct (m2 !! addr_index a) as [[w2' β']|] eqn:Hw2; simplify_equality'.
   destruct (w1' !!{Γ} addr_ref Γ a) as [w1''|] eqn:?; simplify_equality'.
   destruct (w2' !!{Γ} addr_ref Γ a) as [w2''|] eqn:?; simplify_equality'.
-  destruct (Hm1 (addr_index a) w1') as (τ1&?&_),
-    (Hm2 (addr_index a) w2') as (τ2&?&_), Hm as [? _]; auto.
+  destruct (Hm1 (addr_index a) (w1',β)) as (τ1&?&_),
+    (Hm2 (addr_index a) (w2',β')) as (τ2&?&_), Hm as [? _]; auto.
   assert (τ1 = τ2) by eauto using ctree_disjoint_typed_unique.
   simplify_option_equality;
     eauto using ctree_lookup_byte_disjoint, ctree_lookup_disjoint.
@@ -164,12 +166,12 @@ Proof.
   destruct m1 as [m1], m2 as [m2]; simpl.
   intros ? Hm ??. case_option_guard; simplify_equality'.
   specialize (Hm (addr_index a)).
-  destruct (m1 !! (addr_index a)) as [w1'|] eqn:?; simplify_equality'.
-  destruct (m2 !! (addr_index a)) as [w2'|] eqn:?; simplify_equality'; [|done].
+  destruct (m1 !! (addr_index a)) as [[w1' β]|] eqn:?,
+    (m2 !! (addr_index a)) as [[w2' β']|] eqn:?; simplify_equality'; [|done].
   destruct (w1' !!{Γ} addr_ref Γ a) as [w1''|] eqn:?; simplify_equality'.
   destruct (ctree_lookup_subseteq Γ w1' w2' (addr_ref Γ a) w1'')
     as (w2''&?&?); simplify_option_equality; intuition eauto using
-    ctree_lookup_byte_Forall, pbit_unmapped_indetify, ctree_lookup_byte_subseteq.
+    ctree_lookup_byte_Forall, pbit_unmapped_indetify,ctree_lookup_byte_subseteq.
   exfalso; eauto using @ctree_unshared_weaken.
 Qed.
 Lemma cmap_alter_index_type_check Γ m g a w o :
@@ -179,9 +181,9 @@ Proof.
   unfold type_check, index_type_check. destruct m as [m]; simpl. intros ? Hm ??.
   case_option_guard; simplify_equality'.
   destruct (decide (o = addr_index a)); simplify_map_equality'; auto.
-  destruct (m !! addr_index a) as [w'|] eqn:?; simplify_equality'; f_equal.
+  destruct (m !! addr_index a) as [[w' β]|] eqn:?; simplify_equality'; f_equal.
   destruct (w' !!{Γ} addr_ref Γ a) as [w''|] eqn:?; simplify_equality'.
-  destruct (Hm (addr_index a) w') as (τ&?&?&_); auto.
+  destruct (Hm (addr_index a) (w',β)) as (τ&?&?&_); auto.
   destruct (ctree_lookup_Some Γ (CMap m) w' τ (addr_ref Γ a) w'')
     as (σ'&?&?); auto; simplify_type_equality'.
   eapply ctree_alter_type_of_weak; eauto using type_of_typed.
@@ -199,13 +201,15 @@ Lemma cmap_alter_index_alive Γ m g a w o :
   ✓ Γ → ✓{Γ} m → m !!{Γ} a = Some w → ¬ctree_unmapped w →
   index_alive (cmap_alter Γ g a m) o → index_alive m o.
 Proof.
-  destruct m as [m]. intros ? Hm Hw Hunmap (w''&Hw'&Hw''); do 2 red; simpl in *.
-  rewrite lookup_alter_Some in Hw'; destruct Hw' as [(<-&w'&?&->)|[??]]; eauto.
-  exists w'; split; auto; clear Hw''; intros Hw'; destruct Hunmap.
+  destruct m as [m].
+  intros ? Hm Hw Hunmap ([w'' ?]&Hw'&Hw''); do 2 red; simpl in *.
+  rewrite lookup_alter_Some in Hw';
+    destruct Hw' as [(<-&[w' β]&?&FOO)|[??]]; eauto; simplify_equality'.
+  exists (w',β); split; auto; clear Hw''; intros Hw'; destruct Hunmap.
   case_option_guard; simplify_map_equality'.
   destruct (w' !!{Γ} addr_ref Γ a) as [w''|] eqn:?; simplify_equality'.
   assert (ctree_unmapped w'').
-  { destruct (Hm (addr_index a) w') as (τ&?&_); auto.
+  { destruct (Hm (addr_index a) (w',β)) as (τ&?&_); auto.
     destruct (ctree_lookup_Some Γ (CMap m) w' τ
       (addr_ref Γ a) w'') as (τ'&?&?); auto.
     eauto using ctree_lookup_Forall, pbit_unmapped_indetify,
@@ -221,23 +225,23 @@ Lemma cmap_alter_valid Γ m g a w :
   ✓ Γ → ✓{Γ} m → m !!{Γ} a = Some w → (Γ,m) ⊢ g w : type_of w →
   ¬ctree_unmapped (g w) → ✓{Γ} (cmap_alter Γ g a m).
 Proof.
-  intros ? Hm Hw ? Hgw o w''' ?. cut (∃ τ, (Γ,m) ⊢ w''' : τ
+  intros ? Hm Hw ? Hgw o [w''' β] ?. cut (∃ τ, (Γ,m) ⊢ w''' : τ
     ∧ ¬ctree_empty w''' ∧ int_typed (size_of Γ τ) sptrT).
   { intros (τ&?&?&?); exists τ; split_ands;
       eauto using cmap_typed_alter_weaken, type_of_correct. }
   destruct m as [m]; simpl in *; case_option_guard; simplify_equality'.
-  destruct (m !! addr_index a) as [w'|] eqn:?; simplify_equality'.
+  destruct (m !! addr_index a) as [[w' ?]|] eqn:?; simplify_equality'.
   destruct (w' !!{Γ} addr_ref Γ a) as [w''|] eqn:?; simplify_equality'.
-  destruct (decide (addr_index a = o));
-    simplify_map_equality'; [|destruct (Hm o w''') as (τ&?&?&?&?); eauto].
-  destruct (Hm (addr_index a) w') as (τ&?&Hemp&?); auto.
+  destruct (decide (addr_index a = o)); simplify_map_equality';
+    [|destruct (Hm o (w''',β)) as (τ&?&?&?); eauto].
+  destruct (Hm (addr_index a) (w',β)) as (τ&?&Hemp&?); auto.
   exists τ; simplify_option_equality.
   { intuition eauto using ctree_alter_lookup_Forall,
       ctree_alter_typed, @ctree_empty_unmapped. }
   destruct (ctree_lookup_Some Γ (CMap m) w' τ
     (addr_ref Γ a) w'') as (τ'&?&?); auto.
   assert ((Γ,CMap m) ⊢ w : ucharT)
-    by eauto using ctree_lookup_byte_typed; simplify_type_equality.
+    by eauto using ctree_lookup_byte_typed; simplify_type_equality'.
   split_ands; auto.
   { eapply ctree_alter_typed; eauto using ctree_alter_byte_typed,
       type_of_typed, ctree_alter_byte_unmapped. }
@@ -249,7 +253,7 @@ Lemma cmap_alter_freeze Γ q g m a :
 Proof.
   destruct m as [m]; f_equal'. rewrite addr_index_freeze,
     addr_ref_freeze, addr_ref_byte_freeze, ctree_alter_freeze.
-  apply alter_ext; intros; apply ctree_alter_ext; intros.
+  apply alter_ext; intros [??] ?; f_equal'. apply ctree_alter_ext; intros.
   by rewrite (decide_iff _ _ _ _ (addr_is_obj_freeze q a)).
 Qed.
 Lemma cmap_alter_commute Γ g1 g2 m a1 a2 w1 w2 τ1 τ2 :
@@ -263,8 +267,9 @@ Proof.
     intros ? Hm [?|[[-> ?]|(->&Ha&?&?&?)]] ? Hw1 ?? Hw2?; f_equal.
   { by rewrite alter_commute. }
   { rewrite <-!alter_compose.
-    apply alter_ext; simpl; auto using ctree_alter_commute. }
-  rewrite <-!alter_compose. apply alter_ext; intros w Hw; simplify_type_equality'.
+    apply alter_ext; intros [??] ?; f_equal'; auto using ctree_alter_commute. }
+  rewrite <-!alter_compose.
+  apply alter_ext; intros [w β] Hw; f_equal'; simplify_type_equality'.
   repeat case_option_guard; simplify_equality'.
   rewrite Hw in Hw1, Hw2; simplify_equality'.
   rewrite <-!(ctree_alter_freeze _ true _ (addr_ref Γ a1)), !Ha,
@@ -273,7 +278,7 @@ Proof.
     (w !!{Γ} addr_ref Γ a2) as [w2'|] eqn:Hw2'; simplify_option_equality.
   assert (τ1 = ucharT) by intuition eauto using addr_not_obj_type.
   assert (τ2 = ucharT) by intuition eauto using addr_not_obj_type.
-  destruct (Hm (addr_index a2) w) as (τ&?&_); auto.
+  destruct (Hm (addr_index a2) (w,β)) as (τ&?&_); auto.
   assert (w1' = w2') by eauto using ctree_lookup_freeze_proper; subst.
   destruct (ctree_lookup_Some Γ (CMap m) w τ
     (addr_ref Γ a2) w2') as (τ'&_&?); auto.
@@ -285,7 +290,7 @@ Lemma cmap_lookup_alter Γ g m a w :
   cmap_alter Γ g a m !!{Γ} a = Some (g w).
 Proof.
   destruct m as [m]; simpl; intros. case_option_guard; simplify_map_equality'.
-  destruct (m !! addr_index a) as [w'|] eqn:?; simplify_equality'.
+  destruct (m !! addr_index a) as [[w' β]|] eqn:?; simplify_equality'.
   destruct (w' !!{Γ} addr_ref Γ a) as [w''|] eqn:?; simplify_equality'.
   erewrite ctree_lookup_alter by eauto using ctree_lookup_unfreeze; simpl.
   by case_decide; simplify_equality'.
@@ -298,12 +303,12 @@ Lemma cmap_lookup_alter_not_obj Γ g m a w τ :
 Proof.
   destruct m as [m]; simpl; intros ? Hm ?????.
   case_option_guard; simplify_map_equality'.
-  assert (type_of <$> m !! addr_index a = Some (addr_type_object a)).
+  assert (type_of ∘ fst <$> m !! addr_index a = Some (addr_type_object a)).
   { by refine (addr_typed_index Γ (CMap m) a τ _). }
   assert (Γ ⊢ addr_ref Γ a : addr_type_object a ↣ addr_type_base a).
   { eapply addr_typed_ref_typed; eauto. }
-  destruct (m !! addr_index a) as [w'|] eqn:?; simplify_equality'.
-  destruct (Hm (addr_index a) w') as (τ'&?&_); auto.
+  destruct (m !! addr_index a) as [[w' β]|] eqn:?; simplify_equality'.
+  destruct (Hm (addr_index a) (w',β)) as (τ'&?&_); auto.
   destruct (w' !!{Γ} addr_ref Γ a) as [w''|] eqn:?; simplify_equality'.
   destruct (ctree_lookup_Some Γ (CMap m)
     w' τ' (addr_ref Γ a) w'') as (τ''&?&?); auto; simplify_type_equality.
@@ -323,13 +328,13 @@ Proof.
   destruct m as [m]; simpl; intros ? Hm [?|[[-> ?]|(->&Ha&?&?&?)]] ?? Hw2 ??;
     simplify_map_equality; auto.
   { repeat case_option_guard; simplify_equality'; try contradiction.
-    destruct (m !! _) as [w2'|]; simplify_equality'.
+    destruct (m !! _) as [[w2' β]|]; simplify_equality'.
     destruct (w2' !!{Γ} addr_ref Γ a1) as [w1''|] eqn:?,
       (w2' !!{Γ} addr_ref Γ a2) as [w2''|] eqn:?; simplify_equality'.
     by erewrite ctree_lookup_alter_disjoint by eauto. }
   repeat case_option_guard; simplify_type_equality'; try contradiction.
-  destruct (m !! _) as [w|]eqn:?; simplify_equality'.
-  destruct (Hm (addr_index a2) w) as (τ&?&_); auto.
+  destruct (m !! _) as [[w β]|]eqn:?; simplify_equality'.
+  destruct (Hm (addr_index a2) (w,β)) as (τ&?&_); auto.
   destruct (w !!{Γ} addr_ref Γ a1) as [w1'|] eqn:?,
     (w !!{Γ} addr_ref Γ a2) as [w2'|] eqn:?; simplify_equality'.
   assert (w1' = w2') by eauto using ctree_lookup_freeze_proper; subst.
@@ -354,13 +359,13 @@ Proof.
   destruct m1 as [m1], m2 as [m2]; simpl. intros ? Hm1 Hm ????? o.
   specialize (Hm o). case_option_guard; simplify_type_equality'.
   destruct (decide (o = addr_index a)); simplify_map_equality'; [|apply Hm].
-  destruct (m1 !! addr_index a) as [w1'|] eqn:?; simplify_equality'.
+  destruct (m1 !! addr_index a) as [[w1' β]|] eqn:?; simplify_equality'.
   destruct (w1' !!{Γ} addr_ref Γ a) as [w1''|] eqn:?; simplify_equality'.
-  destruct (Hm1 (addr_index a) w1') as (τ&?&_); auto.
+  destruct (Hm1 (addr_index a) (w1',β)) as (τ&?&_); auto.
   destruct (ctree_lookup_Some Γ (CMap m1) w1' τ (addr_ref Γ a) w1'')
     as (τ'&_&?); auto.
   destruct (m2 !! addr_index a) as [w2'|] eqn:?.
-  * destruct Hm as (?&?&?). case_decide; simplify_option_equality.
+  * destruct Hm as (?&?&?&?); case_decide; simplify_option_equality.
     { split_ands; eauto using ctree_alter_disjoint, ctree_alter_lookup_Forall. }
     assert (τ1 = ucharT) by intuition eauto using addr_not_obj_type.
     simplify_equality; split_ands; auto.
@@ -391,13 +396,13 @@ Proof.
   destruct (decide (addr_index a = o)) as [<-|?]; rewrite !lookup_union_with,
     ?lookup_alter, ?lookup_alter_ne, ?lookup_union_with by done; auto.
   specialize (Hm (addr_index a)).
-  destruct (m1 !! addr_index a) as [w1'|] eqn:?,
-    (m2 !! addr_index a); simplify_equality'; f_equal.
+  destruct (m1 !! addr_index a) as [[w1' β]|] eqn:?,
+    (m2 !! addr_index a); simplify_equality'; do 2 f_equal.
   destruct (w1' !!{Γ} addr_ref Γ a) as [w1''|] eqn:?; simplify_equality'.
-  destruct (Hm1 (addr_index a) w1') as (τ&?&_); auto.
+  destruct (Hm1 (addr_index a) (w1',β)) as (τ&?&_); auto.
   destruct (ctree_lookup_Some Γ (CMap m1)
     w1' τ (addr_ref Γ a) w1'') as (τ'&_&?); auto.
-  destruct Hm as (?&?&?). case_decide; simplify_option_equality.
+  destruct Hm as (?&?&?&?); case_decide; simplify_option_equality.
   { eauto using ctree_alter_union. }
   assert (τ1 = ucharT) by intuition eauto using addr_not_obj_type.
   simplify_equality. eapply ctree_alter_union; intuition eauto using
@@ -416,11 +421,11 @@ Proof.
   intros ? Hm ??????. destruct (addr_disjoint_cases Γ m a1 a2 σ1 σ2)
     as [Ha12|[?|[?|(Hidx&s&r1'&i1&r2'&i2&r'&Ha1&Ha2&?)]]]; auto.
   do 3 right. intros g j1 j2.
-  assert (∃ w, cmap_car m !! addr_index a1 = Some w
-    ∧ addr_type_object a1 = type_of w) as (w&?&Hidx1).
+  assert (∃ wβ, cmap_car m !! addr_index a1 = Some wβ
+    ∧ addr_type_object a1 = type_of (wβ.1)) as (w&?&Hidx1).
   { eapply index_typed_alt, addr_typed_index; eauto. }
-  assert (∃ w, cmap_car m !! addr_index a1 = Some w
-    ∧ addr_type_object a2 = type_of w) as (?&?&?); simplify_equality'.
+  assert (∃ wβ, cmap_car m !! addr_index a1 = Some wβ
+    ∧ addr_type_object a2 = type_of (wβ.1)) as (?&?&?); simplify_equality'.
   { rewrite Hidx. eapply index_typed_alt, addr_typed_index; eauto. }
   destruct m as [m]; unfold insertE, cmap_alter, lookupE, cmap_lookup;
     simpl in *; rewrite !addr_index_plus, <-!Hidx; simplify_map_equality'.
@@ -442,11 +447,11 @@ Lemma cmap_refine_index_typed Γ m1 m2 f o1 o2 r τ :
   m1 ⊢ o1 : τ → ∃ τ', m2 ⊢ o2 : τ' ∧ Γ ⊢ r : τ' ↣ τ.
 Proof.
   rewrite index_typed_alt; unfold typed, index_typed,
-    type_check, index_type_check; intros ? (_&_&Hm2&Hm) ? (w1&?&->).
-  destruct (Hm o1 o2 r w1) as (w2&w2'&τ&Ho2&?&?); auto; rewrite Ho2; simpl.
+    type_check, index_type_check; intros ? (_&_&Hm2&Hm) ? ([w1 β]&?&->).
+  destruct (Hm o1 o2 r w1 β) as (w2&w2'&τ&Ho2&?&?&?); auto; rewrite Ho2; simpl.
   assert ((Γ,m1) ⊢ w1 : τ) by eauto using ctree_refine_typed_l.
   assert ((Γ,m2) ⊢ w2' : τ) by eauto using ctree_refine_typed_r.
-  destruct (Hm2 o2 w2) as (τ2&?&_); auto; simplify_type_equality.
+  destruct (Hm2 o2 (w2,β)) as (τ2&?&_); auto; simplify_type_equality.
   exists τ2; split; auto. destruct (ctree_lookup_Some Γ m2 w2 τ2
     (freeze true <$> r) w2') as (τ2'&?&?); simplify_type_equality';
     eauto using ref_typed_freeze_1.
@@ -455,9 +460,9 @@ Lemma cmap_refine_alive Γ m1 m2 f o1 o2 r :
   ✓ Γ → m1 ⊑{Γ,f} m2 → f !! o1 = Some (o2,r) →
   index_alive m1 o1 → index_alive m2 o2.
 Proof.
-  intros ? (_&_&_&Hm) ? (w1&?&Hw1).
-  destruct (Hm o1 o2 r w1) as (w2&w2'&τ&?&?&?); auto.
-  exists w2; split; auto. contradict Hw1; eauto using ctree_lookup_Forall,
+  intros ? (_&_&_&Hm) ? ([w1 β]&?&Hw1).
+  destruct (Hm o1 o2 r w1 β) as (w2&w2'&τ&?&?&?&?); auto.
+  exists (w2,β); split; auto. contradict Hw1; eauto using ctree_lookup_Forall,
     ctree_flatten_refine, pbit_refine_freed_inv.
 Qed.
 Lemma cmap_refine_injective Γ f m1 m2 : m1 ⊑{Γ,f} m2 → mem_inj_injective f.
@@ -471,23 +476,25 @@ Lemma cmap_refine_id Γ m : ✓ Γ → ✓{Γ} m → m ⊑{Γ} m.
 Proof.
   destruct m as [m]; intros ? Hm.
   split; split_ands; auto using mem_inj_id_injective.
-  intros ? o r w ??; simplify_equality'. destruct (Hm o w) as (τ&?&_); auto.
-  exists w w; simplify_type_equality; eauto using ctree_refine_id, type_of_typed.
+  intros ? o r w β ??; simplify_equality'.
+  destruct (Hm o (w,β)) as (τ&?&_); auto.
+  exists w w; simplify_type_equality;
+    eauto 6 using ctree_refine_id, type_of_typed.
 Qed.
 Lemma cmap_refine_compose Γ f1 f2 m1 m2 m3 :
   ✓ Γ → m1 ⊑{Γ,f1} m2 → m2 ⊑{Γ,f2} m3 → m1 ⊑{Γ,f1 ◎ f2} m3.
 Proof.
   intros ? (?&?&?&Hm12) (?&_&?&Hm23); split; split_ands;
     eauto 2 using mem_inj_compose_injective, cmap_refine_injective.
-  intros o1 o3 r w1.
+  intros o1 o3 r w1 β.
   rewrite lookup_mem_inj_compose_Some; intros (o2&r2&r3&?&?&->) Hw1.
-  destruct (Hm12 o1 o2 r2 w1) as (w2&w2'&τ2&?&?&?); auto.
-  destruct (Hm23 o2 o3 r3 w2) as (w3&w3'&τ3&->&?&?); auto.
+  destruct (Hm12 o1 o2 r2 w1 β) as (w2&w2'&τ2&?&?&?&?); auto.
+  destruct (Hm23 o2 o3 r3 w2 β) as (w3&w3'&τ3&->&?&?&?); auto.
   destruct (ctree_lookup_refine Γ f2 m2 m3 w2 w3' τ3
     (freeze true <$> r2) w2') as (w3''&?&Hw23); auto.
-  erewrite ctree_refine_type_of_r in Hw23 by eauto. exists w3 w3''.
+  erewrite ctree_refine_type_of_r in Hw23 by eauto. exists w3 w3'' τ2.
   rewrite fmap_app, ctree_lookup_app; simplify_option_equality.
-  split_ands; eauto using ctree_refine_compose.
+  naive_solver eauto using ctree_refine_compose.
 Qed.
 Lemma cmap_refine_weaken Γ Γ' f f' m1 m2 :
   ✓ Γ → m1 ⊑{Γ,f} m2 → Γ ⊆ Γ' → (∀ o τ, m1 ⊢ o : τ → f !! o = f' !! o) →
@@ -500,10 +507,10 @@ Proof.
   assert (∀ o o2 r τ, m1 ⊢ o : τ → f' !! o = Some (o2,r) →
     f !! o = Some (o2,r)) by (by intros; erewrite Hf by eauto).
   destruct Hm as (?&?&?&Hm); split; split_ands;
-    eauto 2 using cmap_valid_weaken; intros o1 o2 r w1 ??.
+    eauto 2 using cmap_valid_weaken; intros o1 o2 r w1 β ??.
   assert (m1 ⊢ o1 : type_of w1) by (rewrite index_typed_alt; eauto).
-  destruct (Hm o1 o2 r w1) as (w2&w2'&τ&?&?&?); eauto.
-  exists w2 w2' τ; eauto using ctree_refine_weaken, ctree_lookup_weaken.
+  destruct (Hm o1 o2 r w1 β) as (w2&w2'&τ&?&?&?&?); eauto.
+  exists w2 w2' τ; eauto 6 using ctree_refine_weaken, ctree_lookup_weaken.
 Qed.
 Lemma cmap_lookup_refine Γ f m1 m2 a1 a2 w1 τ :
   ✓ Γ → m1 ⊑{Γ,f} m2 → a1 ⊑{Γ,f@m1↦m2} a2 : τ → m1 !!{Γ} a1 = Some w1 →
@@ -514,11 +521,11 @@ Proof.
   assert ((Γ,CMap m2) ⊢ a2 : τ) by eauto using addr_refine_typed_r.
   case_option_guard; simplify_type_equality'.
   rewrite option_guard_True by eauto using addr_strict_refine.
-  destruct (m1 !! addr_index a1) as [w1'|] eqn:?; simplify_equality'.
+  destruct (m1 !! addr_index a1) as [[w1' β]|] eqn:?; simplify_equality'.
   destruct (w1' !!{Γ} addr_ref Γ a1) as [w1''|] eqn:?; simplify_equality'.
   destruct (addr_ref_refine Γ f (CMap m1) (CMap m2) a1 a2 τ) as (r&?&->); auto.
-  destruct (Hm (addr_index a1) (addr_index a2) r w1')
-    as (w2&w2'&τ2&->&Hr&?); auto; csimpl.
+  destruct (Hm (addr_index a1) (addr_index a2) r w1' β)
+    as (w2&w2'&τ2&->&Hr&?&_); auto; csimpl.
   destruct (ctree_lookup_Some Γ (CMap m1) w1' τ2
     (addr_ref Γ a1) w1'') as (σ'&?&?); eauto using ctree_refine_typed_l.
   rewrite ctree_lookup_app, Hr; csimpl.
@@ -528,17 +535,19 @@ Proof.
     case_decide; simplify_equality'.
   { cut (τ = type_of w1); [intros ->; eauto|].
     erewrite <-(addr_is_obj_type_base _ _ a1 τ) by eauto.
-    assert (∃ w, m1 !! addr_index a1 = Some w ∧ addr_type_object a1 = type_of w) 
-      as (?&?&Hidx) by (eapply (index_typed_alt (CMap m1)),
-      addr_typed_index, addr_refine_typed_l; eauto); simplify_type_equality'.
+    assert (∃ wβ, m1 !! addr_index a1 = Some wβ
+      ∧ addr_type_object a1 = type_of (wβ.1)) as (?&?&Hidx)
+      by (eapply (index_typed_alt (CMap m1)),
+        addr_typed_index, addr_refine_typed_l; eauto); simplify_type_equality'.
     eapply ref_set_offset_typed_unique; eauto.
     erewrite <-(ctree_refine_type_of_l _ _ _ _ _ _ τ2) by eauto.
-    rewrite <-Hidx; eauto using addr_typed_ref_base_typed, addr_refine_typed_l. }
+    rewrite <-Hidx; eauto using addr_typed_ref_base_typed,addr_refine_typed_l. }
   case_option_guard; simplify_equality'; rewrite option_guard_True
     by intuition eauto using pbits_refine_unshared, ctree_flatten_refine.
   assert (τ = ucharT) by (intuition eauto using
     addr_not_obj_type, addr_refine_typed_l); subst.
-  erewrite <-addr_ref_byte_refine by eauto. eauto using ctree_lookup_byte_refine.
+  erewrite <-addr_ref_byte_refine by eauto.
+  eauto using ctree_lookup_byte_refine.
 Qed.
 Lemma cmap_alter_refine Γ f g1 g2 m1 m2 a1 a2 w1 w2 τ :
   ✓ Γ → m1 ⊑{Γ,f} m2 → a1 ⊑{Γ,f@m1↦m2} a2 : τ →
@@ -558,12 +567,13 @@ Proof.
   { eapply cmap_alter_valid;
       eauto using pbits_refine_mapped, ctree_flatten_refine.
     simplify_type_equality; eauto using ctree_refine_typed_r. }
-  cut (∀ o3 o4 r4 w3, f !! o3 = Some (o4, r4) →
-    cmap_car (cmap_alter Γ g1 a1 m1) !! o3 = Some w3 → ∃ w4 w4' τ',
-    cmap_car (cmap_alter Γ g2 a2 m2) !! o4 = Some w4 ∧
-    w4 !!{Γ} (freeze true<$>r4) = Some w4' ∧ w3 ⊑{Γ,f@m1↦m2} w4' : τ').
-  { intros help o3 o4 r4 w3 ? Hw3.
-    destruct (help o3 o4 r4 w3) as (w4&w4'&τ'&?&?&?); auto.
+  cut (∀ o3 o4 r4 w3 β, f !! o3 = Some (o4, r4) →
+    cmap_car (cmap_alter Γ g1 a1 m1) !! o3 = Some (w3,β) → ∃ w4 w4' τ',
+    cmap_car (cmap_alter Γ g2 a2 m2) !! o4 = Some (w4,β) ∧
+    w4 !!{Γ} (freeze true<$>r4) = Some w4' ∧ w3 ⊑{Γ,f@m1↦m2} w4' : τ' ∧
+    (β → r4 = [])).
+  { intros help o3 o4 r4 w3 β ? Hw3.
+    destruct (help o3 o4 r4 w3 β) as (w4&w4'&τ'&?&?&?&?); auto.
     exists w4 w4' τ'; split_ands; auto.
     eapply (ctree_refine_weaken _ _ _ _ m1 m2); eauto 1.
     * intros. eapply cmap_alter_index_typed; eauto.
@@ -571,20 +581,23 @@ Proof.
     * intros. eapply cmap_alter_index_typed; eauto.
       by erewrite ctree_refine_type_of_r, type_of_correct by eauto.
     * eauto using cmap_alter_index_alive.
-    * clear dependent o3 o4 r4 w3 τ' w4 w4'. intros o3 o4 r4 ? (w3&?&Hw3).
-      destruct (help o3 o4 r4 w3) as (w4&w4'&τ'&?&?&?); auto.
-      exists w4; split; auto. contradict Hw3; eauto using
+    * clear dependent o3 o4 r4 w3 τ' w4 w4' β.
+      intros o3 o4 r4 ? ([w3 β]&?&Hw3).
+      destruct (help o3 o4 r4 w3 β) as (w4&w4'&τ'&?&?&?&_); auto.
+      exists (w4,β); split; auto. contradict Hw3; eauto using
         ctree_lookup_Forall, pbit_refine_freed_inv, ctree_flatten_refine. }
-  intros o3 o4 r4 w3 ? Hw3. destruct m1 as [m1], m2 as [m2]; simpl in *.
+  intros o3 o4 r4 w3 β ? Hw3. destruct m1 as [m1], m2 as [m2]; simpl in *.
   repeat case_option_guard; simplify_type_equality'.
-  destruct (addr_ref_refine Γ f (CMap m1) (CMap m2) a1 a2 τ) as (r2&?&Hr2); auto.
+  destruct (addr_ref_refine Γ f
+    (CMap m1) (CMap m2) a1 a2 τ) as (r2&?&Hr2); auto.
   rewrite Hr2 in Hw2 |- *; clear Hr2.
-  destruct (m1 !! addr_index a1) as [w1'|] eqn:?; simplify_equality'.
-  destruct (m2 !! addr_index a2) as [w2'|] eqn:?; simplify_equality'.
+  destruct (m1 !! addr_index a1) as [[w1' ?]|] eqn:?; simplify_equality'.
+  destruct (m2 !! addr_index a2) as [[w2' ?]|] eqn:?; simplify_equality'.
   rewrite ctree_lookup_app in Hw2.
   destruct (w1' !!{Γ} addr_ref Γ a1) as [w1''|] eqn:?; simplify_equality'.
   destruct (decide (o3 = addr_index a1)); simplify_map_equality'.
-  * destruct (Hm (addr_index a1) (addr_index a2) r2 w1') as (?&w2''&τ2&?&?&?); auto.
+  * destruct (Hm (addr_index a1) (addr_index a2) r2 w1' β)
+      as (?&w2''&τ2&?&?&?&?); auto.
     destruct (ctree_lookup_refine Γ f (CMap m1) (CMap m2) w1' w2'' τ2
       (addr_ref Γ a1) w1'') as (w2'''&?&?); auto; simplify_map_equality'.
     eexists _, (ctree_alter Γ _ (addr_ref Γ a1) w2''), τ2; split_ands; eauto.
@@ -599,11 +612,11 @@ Proof.
     eapply ctree_alter_refine; eauto using ctree_alter_byte_refine.
     contradict Hgw1. eapply (ctree_alter_byte_unmapped _ _ _ w1'');
       eauto using ctree_alter_lookup_Forall, ctree_refine_typed_l.
-  * destruct (mem_inj_injective_ne f (addr_index a1) (addr_index a2) o3 o4 r2 r4)
-      as [?|[??]]; eauto using cmap_refine_injective;
-      simplify_map_equality'; [eauto|].
-    destruct (Hm o3 (addr_index a2) r4 w3)
-      as (w4''&w4'&τ4&?&?&?); auto; simplify_map_equality'.
+  * destruct (mem_inj_injective_ne f (addr_index a1)
+      (addr_index a2) o3 o4 r2 r4) as [?|[??]];
+      eauto using cmap_refine_injective; simplify_map_equality'; [eauto|].
+    destruct (Hm o3 (addr_index a2) r4 w3 β)
+      as (w4''&w4'&τ4&?&?&?&?); auto; simplify_map_equality'.
     eexists _, w4', τ4; split_ands; eauto.
     by erewrite ctree_alter_app, ctree_lookup_alter_disjoint by
       (eauto; by apply ref_disjoint_freeze_l, ref_disjoint_freeze_r).
