permissions.v
@@ -10,22 +10,17 @@ Concrete permissions are built from more primitive combinators:
   describes that the object has been freed.
 - [lockable]: [Locked] describes that the object has been locked due to
   a sequenced write, and [Unlocked] means that it is not locked
-- [tagged]: [Tagged true] describes that the object has been obtained
-  using [alloc], and [Tagged false] describes that the object is a block
-  scoped variable.
 - [counter] is to account for tokens to keep track of parts of the memory
   that are addresseble.
 *)
-Definition perm := freeable (lockable (tagged (counter Qcanon.Qc) false)).
+Definition perm := freeable (lockable (counter Qcanon.Qc)).
 Instance perm_sep_ops : SeparationOps perm := _.
 Instance perm_sep : Separation perm := _.
 Typeclasses Opaque perm.
 
 Definition perm_freed : perm := Freed.
-Definition perm_full (alloc : bool) : perm :=
-  Available (LUnlocked (Tagged (Counter 0 1) alloc)).
-Definition perm_token : perm :=
-  Available (LUnlocked (Tagged (Counter (-1) ∅) false)).
+Definition perm_full : perm := Available (LUnlocked (Counter 0 1)).
+Definition perm_token : perm := Available (LUnlocked (Counter (-1) ∅)).
 
 Inductive pkind :=
   Freeable | Writable | Readable | Locked | Existing.
@@ -56,11 +51,11 @@ Proof. by repeat split; repeat intros []. Qed.
 Definition perm_kind (x : perm) : option pkind :=
   match x with
   | Freed => None
-  | Available (LUnlocked (Tagged (Counter x' y') alloc)) =>
+  | Available (LUnlocked (Counter x' y')) =>
      if decide (y' = ∅) then
        if decide (x' = 0) then None else Some Existing
      else if decide (y' = 1) then
-       if decide (x' = 0 ∧ alloc = true) then Some Freeable else Some Writable
+       if decide (x' = 0) then Some Freeable else Some Writable
      else Some Readable
   | Available (LLocked _) => Some Locked
   end.
@@ -77,28 +72,26 @@ Definition perm_unlock (x : perm) : perm :=
 
 Inductive perm_kind_view : perm → option pkind → Prop :=
   | perm_kind_None : perm_kind_view Freed None
-  | perm_kind_None' alloc :
-     perm_kind_view (Available (LUnlocked (Tagged (Counter ∅ 0) alloc))) None
-  | perm_kind_Locked x' alloc :
-     perm_kind_view (Available (LLocked (Tagged x' alloc))) (Some Locked)
-  | perm_kind_Existing alloc x' :
-     x' ≠ 0 → perm_kind_view
-      (Available (LUnlocked (Tagged (Counter x' ∅) alloc))) (Some Existing)
-  | perm_kind_Readable alloc x' y' :
-     y' ≠ ∅ → y' ≠ 1 → perm_kind_view
-      (Available (LUnlocked (Tagged (Counter x' y') alloc))) (Some Readable)
+  | perm_kind_None' :
+     perm_kind_view (Available (LUnlocked (Counter ∅ 0))) None
+  | perm_kind_Locked x' :
+     perm_kind_view (Available (LLocked x')) (Some Locked)
+  | perm_kind_Existing x' :
+     x' ≠ 0 →
+     perm_kind_view (Available (LUnlocked (Counter x' ∅))) (Some Existing)
+  | perm_kind_Readable x' y' :
+     y' ≠ ∅ → y' ≠ 1 →
+     perm_kind_view (Available (LUnlocked (Counter x' y'))) (Some Readable)
   | perm_kind_Freeable :
-     perm_kind_view
-      (Available (LUnlocked (Tagged (Counter 0 1) true))) (Some Freeable)
+     perm_kind_view (Available (LUnlocked (Counter 0 1))) (Some Freeable)
   | perm_kind_Writable x' :
-     perm_kind_view
-      (Available (LUnlocked (Tagged (Counter x' 1) false))) (Some Writable)
+     perm_kind_view (Available (LUnlocked (Counter x' 1))) (Some Writable)
   | perm_kind_Writable' x' :
-     x' ≠ 0 → perm_kind_view
-      (Available (LUnlocked (Tagged (Counter x' 1) true))) (Some Writable).
+     x' ≠ 0 →
+     perm_kind_view (Available (LUnlocked (Counter x' 1))) (Some Writable).
 Lemma perm_kind_spec x : perm_kind_view x (perm_kind x).
 Proof.
-  destruct x as [[[]|[[][]]]|]; simpl; repeat case_decide;
+  destruct x as [[[]|[]]|]; simpl; repeat case_decide;
     intuition; simplify_equality'; constructor; auto.
 Qed.
 Arguments perm_kind _ : simpl never.
@@ -107,32 +100,32 @@ Lemma perm_freed_valid : sep_valid perm_freed.
 Proof. done. Qed.
 Lemma perm_kind_Some_not_freed k x : Some k ⊆ perm_kind x → x ≠ perm_freed.
 Proof. intros Hk ->; inversion Hk. Qed.
-Lemma perm_full_valid alloc : sep_valid (perm_full alloc).
-Proof. by compute; intuition. Qed.
+Lemma perm_full_valid : sep_valid perm_full.
+Proof. done. Qed.
 Lemma perm_token_valid : sep_valid perm_token.
 Proof. done. Qed.
 Lemma perm_lock_valid x :
   sep_valid x → Some Writable ⊆ perm_kind x → sep_valid (perm_lock x).
 Proof. destruct (perm_kind_spec x); repeat sep_unfold; intuition. Qed.
 Lemma perm_lock_mapped x : sep_unmapped (perm_lock x) → sep_unmapped x.
-Proof. destruct x as [[[]|[[][]]]|]; repeat sep_unfold; intuition. Qed.
+Proof. destruct x as [[[]|[]]|]; repeat sep_unfold; intuition. Qed.
 Lemma perm_lock_unshared x : sep_unshared x → sep_unshared (perm_lock x).
-Proof. destruct x as [[[[][]]|[[][]]]|]; repeat sep_unfold; intuition. Qed.
+Proof. destruct x as [[[]|[]]|]; repeat sep_unfold; intuition. Qed.
 Lemma perm_unlock_lock x :
   sep_valid x → Some Writable ⊆ perm_kind x → perm_unlock (perm_lock x) = x.
 Proof. by destruct (perm_kind_spec x). Qed.
 Lemma perm_unlock_valid x : sep_valid x → sep_valid (perm_unlock x).
-Proof. destruct x as [[[[][]]|[[][]]]|]; repeat sep_unfold; naive_solver. Qed.
+Proof. destruct x as [[[]|[]]|]; repeat sep_unfold; naive_solver. Qed.
 Lemma perm_unlock_unmapped x : sep_unmapped x → sep_unmapped (perm_unlock x).
-Proof. destruct x as [[[[][]]|[[][]]]|]; repeat sep_unfold; intuition. Qed.
+Proof. destruct x as [[[]|[]]|]; repeat sep_unfold; intuition. Qed.
 Lemma perm_unlock_mapped x :
   sep_valid x → sep_unmapped (perm_unlock x) → sep_unmapped x.
-Proof. destruct x as [[[[][]]|[[][]]]|]; repeat sep_unfold; intuition. Qed.
+Proof. destruct x as [[[]|[]]|]; repeat sep_unfold; intuition. Qed.
 Lemma perm_unlock_unshared x : sep_unshared x → sep_unshared (perm_unlock x).
-Proof. destruct x as [[[[][]]|[[][]]]|]; repeat sep_unfold; intuition. Qed.
+Proof. destruct x as [[[]|[]]|]; repeat sep_unfold; intuition. Qed.
 Lemma perm_unlock_shared x :
   sep_valid x → sep_unshared (perm_unlock x) → sep_unshared x.
-Proof. destruct x as [[[[][]]|[[][]]]|]; repeat sep_unfold; intuition. Qed.
+Proof. destruct x as [[[]|[]]|]; repeat sep_unfold; intuition. Qed.
 Lemma perm_unshared x :
   sep_valid x → Some Locked ⊆ perm_kind x → sep_unshared x.
 Proof. destruct (perm_kind_spec x); repeat sep_unfold; intuition. Qed.
@@ -159,9 +152,8 @@ Lemma perm_splittable_existing x :
   sep_valid x → perm_kind x = Some Existing → sep_splittable x.
 Proof. by destruct (perm_kind_spec x); repeat sep_unfold. Qed.
 
-Lemma perm_kind_full alloc :
-  perm_kind (perm_full alloc) = Some (if alloc then Freeable else Writable).
-Proof. by destruct alloc. Qed.
+Lemma perm_kind_full : perm_kind perm_full = Some Freeable.
+Proof. done. Qed.
 Lemma perm_kind_lock x :
   sep_valid x → Some Writable ⊆ perm_kind x →
   perm_kind (perm_lock x) = Some Locked.
@@ -191,7 +183,7 @@ Lemma perm_kind_difference_token x :
                                end.
 Proof.
   rewrite strict_spec_alt.
-  destruct (perm_kind_spec x) as [| | |? y| | | |y]; repeat sep_unfold;
+  destruct (perm_kind_spec x) as [| | |y| | |y|y]; repeat sep_unfold;
     unfold perm_kind; simpl; intros [? Hneq]; auto.
   * assert (¬0 ≤ -1) by (by intros []); intuition.
   * assert (y ≤ -1 → y ≤ 0) by (by intros; transitivity (-1)). 
@@ -201,7 +193,9 @@ Proof.
       symmetry. unfold perm_token; repeat f_equal; intuition. }
     by rewrite decide_False by done.
   * by change (-0) with 0; rewrite Qcplus_0_r, !decide_False by done.
-  * by rewrite decide_False by (by intros []).
+  * assert (y --1 = 0 → 0 ≤ y → False).
+    { rewrite (Qcplus_le_mono_r _ _ (--1)). by intros -> []. }
+    by rewrite decide_False by intuition eauto.
   * assert (y --1 = 0 → 0 ≤ y → False).
     { rewrite (Qcplus_le_mono_r _ _ (--1)). by intros -> []. }
     by rewrite decide_False by intuition eauto.
